src/SlabsAlloc.fsti
@@ -42,5 +42,10 @@ val allocate_slab
   )
   (requires fun _ -> True)
   (ensures fun _ r _ ->
-    not (A.is_null r) ==> A.length r == U32.v size_class
+    not (A.is_null r) ==> (
+      A.length r == U32.v size_class /\
+      same_base_array r slab_region /\
+      A.offset (A.ptr_of r) - A.offset (A.ptr_of slab_region) >= 0 /\
+      ((A.offset (A.ptr_of r) - A.offset (A.ptr_of slab_region)) % U32.v page_size) % (U32.v size_class) == 0
+    )
   )
